SATnat_real.v
@@ -1,0 +1,463 @@
+
+Require Import ZF ZFpairs ZFsum ZFord ZFfix ZFind_nat Sat SATtypes.
+Require Import ZFlambda.
+Require Import Lambda.
+Module Lc:=Lambda.
+
+Set Implicit Arguments.
+
+(** NAT *)
+
+Definition fNAT (A:set->SAT) : set->SAT :=
+  sumReal (fun _ => unitSAT) A.
+
+Lemma fNAT_morph :
+   Proper ((eq_set ==> eqSAT) ==> eq_set ==> eqSAT) fNAT.
+do 3 red; intros.
+unfold fNAT.
+unfold sumReal.
+apply interSAT_morph.
+apply indexed_relation_id.
+intros.
+apply prodSAT_morph.
+ unfold depSAT.
+ apply interSAT_morph_subset; intros; auto with *.
+ rewrite H0; reflexivity.
+
+ apply prodSAT_morph; auto with *.
+ unfold depSAT.
+ apply interSAT_morph_subset; simpl; intros; auto with *.
+  rewrite H0; reflexivity.
+
+  apply prodSAT_morph; auto with *.
+Qed.
+Hint Resolve fNAT_morph.
+
+Lemma fNAT_irrel (R R' : set -> SAT) (o : set) :
+ isOrd o ->
+ (forall x x' : set, x ∈ TI NATf o -> x == x' -> eqSAT (R x) (R' x')) ->
+ forall x x' : set,
+ x ∈ TI NATf (osucc o) -> x == x' -> eqSAT (fNAT R x) (fNAT R' x').
+intros.
+unfold fNAT.
+apply interSAT_morph.
+apply indexed_relation_id; intro C.
+apply prodSAT_morph.
+ apply interSAT_morph_subset; simpl; intros; auto with *.
+ rewrite H2; reflexivity.
+
+ apply prodSAT_morph; auto with *.
+ apply interSAT_morph_subset; simpl; intros; auto with *.
+  rewrite H2; reflexivity.
+
+  apply prodSAT_morph; auto with *.
+  apply H0; auto with *.
+  rewrite TI_mono_succ in H1; auto.
+  rewrite Px in H1; apply sum_inv_r in H1; trivial.
+Qed.
+
+Lemma Real_ZERO_gen A :
+  inSAT (INL ID) (fNAT A ZERO).
+apply Real_inl.
+ do 2 red; reflexivity.
+
+ apply ID_intro.
+Qed.
+
+Lemma Real_SUCC_gen A n t :
+  Proper (eq_set==>eqSAT) A ->
+  inSAT t (A n) ->
+  inSAT (INR t) (fNAT A (SUCC n)).
+intros.
+apply Real_inr; trivial.
+Qed.
+
+Lemma Real_NATCASE_gen X A C n nt ft gt:
+  Proper (eq_set ==> eqSAT) C ->
+  n ∈ NATf X ->
+  inSAT nt (fNAT A n) ->
+  inSAT ft (C ZERO) ->
+  inSAT gt (depSAT (fun x => x ∈ X) (fun x => prodSAT (A x) (C (SUCC x)))) ->
+  inSAT (Lc.App2 nt (Lc.Abs (Lc.lift 1 ft)) gt) (C n).
+intros Cm nty nreal freal greal.
+apply Real_sum_case with ZFind_basic.UNIT X n (fun _ => unitSAT) A; trivial.
+ apply depSAT_intro.
+  apply Lc.sn_abs.
+  apply Lc.sn_lift.
+  apply sat_sn in freal; trivial.
+
+  intros.
+  rewrite H in nty; apply sum_inv_l in nty.
+  apply ZFind_basic.unit_elim in nty.
+  rewrite nty in H.
+  apply prodSAT_intro; intros.
+  unfold Lc.subst; rewrite Lc.simpl_subst; auto.
+  rewrite Lc.lift0; trivial.
+  rewrite H; trivial.
+
+ apply depSAT_intro.
+  apply sat_sn in greal; trivial.
+
+  intros.
+  rewrite H in nty; apply sum_inv_r in nty.
+  apply prodSAT_intro'; intros.
+  rewrite H.
+  apply prodSAT_elim with (2:=H0).
+  apply depSAT_elim with (P:=fun x => x ∈ X)(x:=x) in greal; trivial.
+Qed.
+
+Definition fNATi o := tiSAT NATf fNAT o.
+
+Instance fNATi_morph :
+  Proper (eq_set ==> eq_set ==> eqSAT) fNATi.
+apply tiSAT_morph; auto.
+Qed.
+
+Lemma fNATi_mono o1 o2:
+  isOrd o1 ->
+  isOrd o2 ->
+  o1 ⊆ o2 ->
+  forall x,
+  x ∈ NATi o1 ->
+  eqSAT (fNATi o1 x) (fNATi o2 x).
+intros.
+apply tiSAT_mono; trivial.
+intros; apply fNAT_irrel with (o:=o'); trivial.
+Qed.
+
+Lemma fNATi_succ_eq o x :
+  isOrd o ->
+  x ∈ NATi (osucc o) ->
+  eqSAT (fNATi (osucc o) x) (fNAT (fNATi o) x).
+intros.
+apply tiSAT_succ_eq; auto.
+intros; apply fNAT_irrel with (o:=o'); trivial.
+Qed.
+
+Lemma fNATi_fix x :
+  x ∈ NAT ->
+  eqSAT (fNATi omega x) (fNAT (fNATi omega) x).
+intros.
+apply tiSAT_eq; auto with *.
+intros; apply fNAT_irrel with (o:=o'); trivial.
+Qed.
+
+Lemma Real_ZERO o :
+  isOrd o ->
+  inSAT (INL ID) (fNATi (osucc o) ZERO).
+intros.
+rewrite fNATi_succ_eq; trivial.
+ apply Real_ZERO_gen.
+
+ apply ZEROi_typ; trivial.
+Qed.
+
+Lemma Real_SUCC o n t :
+  isOrd o ->
+  n ∈ NATi o ->
+  inSAT t (fNATi o n) ->
+  inSAT (INR t) (fNATi (osucc o) (SUCC n)).
+intros.
+rewrite fNATi_succ_eq; trivial.
+ apply Real_inr; trivial.
+ apply fNATi_morph; reflexivity.
+
+ apply SUCCi_typ; trivial.
+Qed.
+
+
+Lemma Real_NATCASE o C n nt ft gt:
+  isOrd o ->
+  Proper (eq_set ==> eqSAT) C ->
+  n ∈ NATi (osucc o) ->
+  inSAT nt (fNATi (osucc o) n) ->
+  inSAT ft (C ZERO) ->
+  inSAT gt (depSAT (fun x => x ∈ NATi o) (fun x => prodSAT (fNATi o x) (C (SUCC x)))) ->
+  inSAT (Lc.App2 nt (Lc.Abs (Lc.lift 1 ft)) gt) (C n).
+intros oo Cm nty nreal freal greal.
+rewrite fNATi_succ_eq in nreal; trivial.
+unfold NATi in nty; rewrite TI_mono_succ in nty; auto.
+apply Real_NATCASE_gen with (2:=nty) (3:=nreal); auto.
+Qed.
+
+(* TODO: reduction of NCASE *)
+
+(** * Structural fixpoint: *)
+
+(** NATFIX m n --> m (NATFIX m) n when n is a (sum) constructor.
+   let G m := "\n. (match n with inl _ => m | inr _ => m end) m n"
+   let G m := \n. n (\_.m) (\_.m) m n
+    G m -/-> ; G m (inl a) --> m m (inl a); G m (inr b) --> m m (inr b)
+   NATFIX m n := G (\x. m (G x)) n
+     --> (\x. m (G x)) (\x. m (G x)) n
+     --> m (G (\x. m (G x))) n == m (NATFIX m) n
+ *)
+
+Definition guard_sum m :=
+  Lc.Abs (Lc.App2 (Lc.App2 (Lc.Ref 0) (Lc.Abs (Lc.lift 2 m)) (Lc.Abs (Lc.lift 2 m))) (Lc.lift 1 m) (Lc.Ref 0)).
+
+(** (G m n) reduces to (m m n) when n is a constructor. Note that
+    n need not be closed. *)
+Lemma G_sim : forall m n,
+  (exists t c, (c=0\/c=1) /\ n = Lc.Abs (Lc.Abs (Lc.App (Lc.Ref c) t))) ->
+  Lc.redp (Lc.App (guard_sum m) n) (Lc.App2 m m n).
+intros m n (t,(c,(eqc,eqn))).
+unfold guard_sum.
+eapply t_trans.
+ apply t_step.
+ apply Lc.beta.
+unfold Lc.subst; simpl.
+repeat rewrite Lc.simpl_subst; auto.
+repeat rewrite Lc.lift0.
+apply Lc.redp_app_l.
+apply Lc.redp_app_l.
+rewrite eqn.
+eapply t_trans.
+ apply t_step.
+ apply Lc.app_red_l.
+ apply Lc.beta.
+destruct eqc; subst c.
+ unfold Lc.subst; simpl.
+ eapply t_trans.
+  apply t_step.
+  apply Lc.beta.
+ unfold Lc.subst; simpl.
+ rewrite Lc.lift0.
+ apply t_step.
+ apply Lc.red1_beta.
+ unfold Lc.subst; rewrite Lc.simpl_subst; auto.
+ rewrite Lc.lift0; trivial.
+
+ unfold Lc.subst; simpl.
+ eapply t_trans.
+  apply t_step.
+  apply Lc.beta.
+ unfold Lc.subst; simpl; rewrite Lc.simpl_subst_rec; auto.
+ rewrite Lc.lift_rec0.
+ apply t_step.
+ apply Lc.red1_beta.
+ unfold Lc.subst; rewrite Lc.simpl_subst; auto.
+ rewrite Lc.lift0; trivial.
+Qed.
+
+(*
+Definition guard_couple m :=
+  Lc.Abs (Lc.App2 (Lc.App (Lc.Ref 0) (Lc.Abs (Lc.Abs (Lc.lift 3 m)))) (Lc.lift 1 m) (Lc.Ref 0)).
+
+(** (G m n) reduces to (m m n) when n is a constructor. Note that
+    n need not be closed. *)
+Lemma G_sim : forall m n,
+  (exists t1 t2, n = Lc.Abs (Lc.App2 (Lc.Ref 0) t1 t2)) ->
+  Lc.redp (Lc.App (guard_couple m) n) (Lc.App2 m m n).
+intros m n (t1,(t2,eqn)).
+unfold guard_couple.
+eapply t_trans.
+ apply t_step.
+ apply Lc.beta.
+unfold Lc.subst; simpl.
+repeat rewrite Lc.simpl_subst; auto.
+repeat rewrite Lc.lift0.
+apply Lc.redp_app_l.
+apply Lc.redp_app_l.
+rewrite eqn.
+eapply t_trans.
+ apply t_step.
+ apply Lc.beta.
+unfold Lc.subst; simpl.
+rewrite Lc.lift0.
+eapply t_trans.
+ apply t_step.
+ apply Lc.app_red_l.
+ apply Lc.beta.
+unfold Lc.subst; simpl.
+rewrite Lc.simpl_subst; auto.
+apply t_step.
+apply Lc.red1_beta.
+unfold Lc.subst; simpl.
+rewrite Lc.simpl_subst; auto.
+rewrite Lc.lift0; trivial.
+Qed.
+*)
+
+Lemma G_sat A k m t X :
+  k ∈ NAT ->
+  inSAT t (fNAT A k) ->
+  inSAT (Lc.App2 m m t) X ->
+  inSAT (Lc.App (guard_sum m) t) X.
+intros.
+unfold guard_sum.
+apply inSAT_exp; intros.
+ right; apply sat_sn in H0; trivial.
+unfold Lc.subst; simpl Lc.subst_rec.
+repeat rewrite Lc.simpl_subst; auto.
+repeat rewrite Lc.lift0.
+revert X H1; apply inSAT_context.
+apply inSAT_context.
+intros.
+apply Real_NATCASE_gen with (X:=NAT) (A:=A) (C:=fun _ => S) (n:=k); auto.
+ do 2 red; reflexivity.
+
+ rewrite NAT_eq in H; trivial.
+
+ apply depSAT_intro; intros.
+  apply Lc.sn_abs.
+  apply Lc.sn_lift.
+  apply sat_sn in H1; trivial.
+
+  apply prodSAT_intro; intros.
+  unfold Lc.subst; simpl Lc.subst_rec.
+  rewrite Lc.simpl_subst; auto.
+  rewrite Lc.lift0; trivial.
+Qed.
+
+Lemma sn_G_inv m : Lc.sn (guard_sum m) -> Lc.sn m.
+intros.
+unfold guard_sum in H.
+eapply subterm_sn in H;[|constructor].
+eapply subterm_sn in H;[|apply sbtrm_app_l].
+eapply subterm_sn in H;[|apply sbtrm_app_r].
+apply sn_lift_inv with (1:=H) (2:=eq_refl).
+Qed.
+
+
+Definition NATFIX m :=
+  guard_sum (Lc.Abs (Lc.App  (Lc.lift 1 m) (guard_sum (Lc.Ref 0)))).
+
+(** NATFIX reduces as a fixpoint combinator when applied to a constructor *)
+Lemma NATFIX_sim : forall m n,
+  (exists t c, (c=0\/c=1) /\ n = Lc.Abs (Lc.Abs (Lc.App (Lc.Ref c) t))) ->
+  Lc.redp (Lc.App (NATFIX m) n) (Lc.App2 m (NATFIX m) n).
+intros.
+unfold NATFIX at 1.
+eapply t_trans.
+ apply G_sim; trivial.
+apply Lc.redp_app_l.
+apply t_step.
+apply Lc.red1_beta.
+set (t1 := Lc.Abs (Lc.App (Lc.lift 1 m) (guard_sum (Lc.Ref 0)))).
+unfold Lc.subst; simpl.
+rewrite Lc.simpl_subst; auto.
+rewrite Lc.lift0.
+reflexivity.
+Qed.
+
+(** The guard is needed mainly here: NATFIX m does not reduce *)
+Lemma sn_natfix o m X B:
+  isOrd o ->
+  inSAT m (interSAT (fun o':{o'|o' ∈ osucc o} => let o1:=proj1_sig o' in
+        prodSAT (depSAT (fun n => n ∈ NATi o1) (fun n => prodSAT (fNATi o1 n) (X o1 n))) (B o'))) ->
+  sn (NATFIX m).
+intros.
+assert (empty ∈ osucc o).
+ apply isOrd_plump with o; auto with *.
+  red; intros.
+  apply empty_ax in H1; contradiction.
+  apply lt_osucc; trivial.
+apply interSAT_elim with (x:=exist (fun o'=>o'∈ osucc o) empty H1) in H0.
+simpl proj1_sig in H0.
+unfold NATFIX.
+assert (sn (Lc.Abs (Lc.App (Lc.lift 1 m) (guard_sum (Lc.Ref 0))))).
+ apply sn_abs.
+ assert (inSAT (guard_sum (Lc.Ref 0)) (depSAT(fun n => n ∈ NATi empty) (fun n => prodSAT (fNATi empty n) (X empty n)))).
+  apply depSAT_intro; intros.
+   apply sn_abs.
+   constructor; intros.
+   apply nf_norm in H2; try contradiction.
+   repeat constructor.
+
+   apply prodSAT_intro'; intros.
+   eapply G_sat with (A:=fNATi empty) (k:=x).
+    revert H2; apply NATi_NAT; auto with *.
+
+    unfold fNATi.
+    rewrite <- tiSAT_succ_eq; auto.
+     2:intros; apply fNAT_irrel with (o:= o'); trivial.
+     2:revert H2; apply TI_incl; auto.
+    rewrite fNATi_mono with (o2:=osucc empty) in H3; auto.
+    red; intros.
+    apply empty_ax in H4; contradiction.
+
+    apply prodSAT_elim with (A:=snSAT).
+    2:apply sat_sn in H3; trivial.
+    apply prodSAT_elim with (A:=snSAT).
+    apply varSAT.
+    apply varSAT.
+
+ specialize prodSAT_elim with (1:=H0)(2:=H2); intro.
+ apply sat_sn in H3; trivial.
+ apply sn_subst with (Ref 0).
+ unfold Lc.subst; simpl.
+ rewrite simpl_subst; auto.
+ rewrite lift0; auto.
+
+apply sn_abs.
+apply prodSAT_elim with (A:=snSAT) (B:=snSAT).
+2:simpl; auto with *.
+apply prodSAT_elim with (A:=snSAT).
+ apply prodSAT_elim with (A:=snSAT).
+  apply prodSAT_elim with (A:=snSAT).
+   apply varSAT.
+   apply sn_abs; apply sn_lift; trivial.
+  apply sn_abs; apply sn_lift; trivial.
+ apply sn_lift; trivial.
+Qed.
+
+
+Lemma NATFIX_sat : forall o m X,
+  isOrd o ->
+  (forall y y' n, isOrd y -> isOrd y' -> y ⊆ y' -> y' ⊆ o -> n ∈ NATi y ->
+   inclSAT (X y n) (X y' n)) ->
+  inSAT m (interSAT (fun o':{o'|o' ∈ osucc o} => let o1:=proj1_sig o' in let o2 := osucc o1 in
+        prodSAT (depSAT (fun n => n ∈ NATi o1) (fun n => prodSAT (fNATi o1 n) (X o1 n)))
+                (depSAT (fun n => n ∈ NATi o2) (fun n => prodSAT (fNATi o2 n) (X o2 n))))) ->
+  inSAT (NATFIX m) (depSAT (fun n => n ∈ NATi o) (fun n => prodSAT (fNATi o n) (X o n))).
+intros o m X oo Xmono msat.
+elim oo using isOrd_ind; intros.
+apply depSAT_intro.
+ apply sn_natfix with (o:=o) (X:=X) (2:=msat); trivial.
+
+intros x i.
+assert (tyx : x ∈ NAT).
+ apply NATi_NAT with y; trivial.
+apply TI_elim in i; auto with *.
+destruct i as (z,?,?).
+assert (zo : isOrd z).
+ apply isOrd_inv with y; trivial.
+unfold NATFIX.
+rewrite <- ZFfix.TI_mono_succ in H3; auto with *.
+apply prodSAT_intro'.
+intros t tty.
+assert (tty' : inSAT t (fNAT (fNATi z) x)).
+ rewrite <- fNATi_succ_eq; trivial.
+ rewrite fNATi_mono with (o2:=y); auto.
+ red; intros.
+ apply isOrd_plump with z; trivial.
+  apply isOrd_inv with (osucc z); auto.
+  apply olts_le in H4; trivial.
+apply G_sat with (2:=tty'); trivial.
+eapply inSAT_context; intros.
+ apply inSAT_exp.
+  left; simpl.
+  apply Bool.orb_true_r.
+
+  unfold Lc.subst; simpl Lc.subst_rec.
+  repeat rewrite Lc.simpl_subst; auto.
+  rewrite Lc.lift0.
+  change (inSAT (Lc.App m (NATFIX m)) S).
+  eexact H4.
+rewrite <- fNATi_succ_eq in tty'; trivial.
+apply Xmono with (osucc z); eauto using isOrd_inv.
+ red; intros.
+ apply isOrd_plump with z; trivial.
+  eauto using isOrd_inv.
+  apply olts_le; trivial.
+apply prodSAT_elim with (A:=fNATi (osucc z) x); trivial.
+assert (z ∈ osucc o).
+ apply isOrd_trans with o; auto.
+ apply H0; trivial.
+apply interSAT_elim with (x:=exist (fun o'=>o' ∈ osucc o) z H4) in msat.
+simpl proj1_sig in msat.
+specialize H1 with (1:=H2).
+specialize prodSAT_elim with (1:=msat) (2:=H1); intro.
+apply (depSAT_elim x H5); trivial.
+Qed.
